**Solution.**

a\) First calculate the right-hand side of the equation.

For $i = j$,

$$
\begin{align*}
p_{ij}\left(t_{1}\right)p_{ji}\left(t_{2}\right) &= \left( \frac{1}{4}+\frac{3}{4}e^{-4\lambda t_{1}} \right)\left( \frac{1}{4} + \frac{3}{4}e^{-4\lambda t_{2}} \right) \\
&= \frac{1}{16}\left(1+3e^{-4\lambda t_{1}} + 3e^{-4\lambda t_{2}} + 9e^{-4\lambda\left( t_{1} + t_{2} \right)} \right).
\end{align*}
$$

For $i \neq j$,

$$\begin{align*}
p_{ij}\left( t_{1} \right)p_{ji}\left( t_{2} \right) &= \left( \frac{1}{4} - \frac{1}{4}e^{-4\lambda t_{1}} \right)\left( \frac{1}{4} - \frac{1}{4}e^{-4\lambda t_{2}} \right) \\
&= \frac{1}{16}\left( 1 - e^{-4\lambda t_{1}} - e^{-4\lambda t_{2}} + e^{-4\lambda\left( t_{1} + t_{2} \right)} \right).
\end{align*}$$

Hence,

$$
p_{ij} \left( t_{1} \right) p_{ji}\left( t_{2} \right) =
\begin{cases}
\frac{1}{16}\left( 1 + 3e^{- 4\lambda t_{1}} + 3e^{- 4\lambda t_{2}} + 9e^{- 4\lambda\left( t_{1} + t_{2} \right)} \right), & i = j \\
\frac{1}{16}\left( 1 - e^{- 4\lambda t_{1}} - e^{- 4\lambda t_{2}} + e^{- 4\lambda\left( t_{1} + t_{2} \right)} \right), & i \neq j
\end{cases}
$$

It follows that

$$
\begin{align*}
&p_{TT}\left( t_{1} \right)p_{TT}\left( t_{2} \right) + p_{TC}\left( t_{1} \right)p_{CT}\left( t_{2} \right) + p_{TA}\left( t_{1} \right)p_{AT}\left( t_{2} \right) + p_{TG}\left( t_{1} \right)p_{GT}\left( t_{2} \right) \\
&= \frac{1}{16}\left( 1 + 3e^{- 4\lambda t_{1}} + 3e^{- 4\lambda t_{2}} + 9e^{- 4\lambda\left( t_{1} + t_{2} \right)} \right) \\
&\quad + 3 \times \frac{1}{16}\left( 1 - e^{- 4\lambda t_{1}} - e^{- 4\lambda t_{2}} + e^{- 4\lambda\left( t_{1} + t_{2} \right)} \right) \\
&= \frac{1}{4} + \frac{3}{4}e^{- 4\lambda\left( t_{1} + t_{2} \right)} \\
&= p_{TT}\left( t_{1} + t_{2} \right).
\end{align*}
$$

b) It follows that

$$
\begin{align*}
&p_{TT}(t_{1})p_{TC}(t_{2}) + p_{TC}(t_{1})p_{CC}(t_{2}) + p_{TA}(t_{1})p_{AT}(t_{2}) + p_{TG}(t_{1})p_{GT}(t_{2}) \\
&= \left(\frac{1}{4} + \frac{3}{4}e^{-4\lambda t_{1}}\right)\left(\frac{1}{4} - \frac{1}{4}e^{-4\lambda t_{2}}\right) \\
&\quad + \left(\frac{1}{4} - \frac{1}{4}e^{-4\lambda t_{1}}\right)\left(\frac{1}{4} + \frac{3}{4}e^{-4\lambda t_{2}}\right) \\
&\quad + 2 \times \left(\frac{1}{4} - \frac{1}{4}e^{-4\lambda t_{1}}\right)\left(\frac{1}{4} - \frac{1}{4}e^{-4\lambda t_{2}}\right) \\
&= \frac{1}{16}\left[ \left(1 - e^{-4\lambda t_{2}} + 3e^{-4\lambda t_{1}} - 3e^{-4\lambda(t_{1} + t_{2})}\right) \right. \\
&\quad + \left(1 - e^{-4\lambda t_{1}} + 3e^{-4\lambda t_{2}} - 3e^{-4\lambda(t_{1} + t_{2})}\right) \\
&\quad + \left. 2 \times \left(1 - e^{-4\lambda t_{1}} - e^{-4\lambda t_{2}} + e^{-4\lambda(t_{1} + t_{2})}\right) \right] \\
&= \frac{1}{4} - \frac{1}{4}e^{-4\lambda(t_{1} + t_{2})} \\
&= p_{TC}(t_{1} + t_{2}).
\end{align*}
$$


